Update for new MetaCoq with flag in evaluation relation
Update for the new MetaCoq version that has a flag that decides whether
matches on boxes can be done. The new relation also requires information
about inductives to be present to determine whether matches are
propositional, so because of this our erasure also needed to change a
bit. In particular, trans_env now has a straightforward translation for
each declaration type.

This should allow us to use MetaCoq's box optimization in a follow-up
change.

extraction/theories/OptimizeCorrectness.v
@@ -27,108 +27,28 @@ Import Erasure.
 Import ExAst.
 Import ConCert.Extraction.Aux.
 
-(* We have our own environment which is different from MetaCoq's erased environment
-   (it includes more information and a different treatment of types).
-   To reconcile this, we map our environments to theirs, but the treatment of types
-   remains different. However, MetaCoq does not actually use information about types
-   for anything during evaluation, so we just filter them out. This is justified
-   by the following lemmas. *)
-Definition is_constant (decl : EAst.global_decl) : bool :=
-  match decl with
-  | EAst.ConstantDecl _ => true
-  | _ => false
-  end.
-
-Definition only_constants (Σ : EAst.global_context) : EAst.global_context :=
-  filter (is_constant ∘ snd) Σ.
-
-Lemma declared_constant_only_constants Σ kn decl :
-  ETyping.declared_constant Σ kn decl ->
-  ETyping.declared_constant (only_constants Σ) kn decl.
+Lemma lookup_env_trans_env Σ kn :
+  ETyping.lookup_env (trans_env Σ) kn =
+  option_map trans_global_decl (lookup_env Σ kn).
 Proof.
-  unfold ETyping.declared_constant.
-  intros lookup_decl.
-  induction Σ; [easy|].
-  destruct a as (kn' & decl').
-  cbn in *.
-  destruct (is_constant decl') eqn:isconst.
-  - cbn in *.
-    destruct (kername_eq_dec _ _) as [<-|?]; easy.
-  - apply IHΣ.
-    destruct (kername_eq_dec _ _).
-    + inversion lookup_decl; subst; easy.
-    + auto.
-Qed.
-
-Lemma eval_only_constants Σ s t :
-  Σ e⊢ s ▷ t ->
-  only_constants Σ e⊢ s ▷ t.
-Proof.
-  induction 1; eauto using eval, declared_constant_only_constants.
-Qed.
-
-Definition trans_cst (cst : constant_body) : EAst.constant_body :=
-  {| EAst.cst_body := cst_body cst |}.
-
-(* Translation from our global environment into MetaCoq's global environment.
-   We only translate constants which is justified by the proof above. *)
-Definition trans_env (Σ : global_env) : EAst.global_context :=
-  let map_decl kn (decl : global_decl) : list (kername * EAst.global_decl) :=
-      match decl with
-      | ConstantDecl cst => [(kn, EAst.ConstantDecl (trans_cst cst))]
-      | InductiveDecl _ => []
-      | TypeAliasDecl o =>
-        [(kn, EAst.ConstantDecl
-                {| EAst.cst_body := option_map (fun _ => tBox) o |})]
-      end in
-  flat_map (fun '(kn, _, decl) => map_decl kn decl) Σ.
-
-Lemma declared_constant_trans Σ kn cst :
-  ETyping.declared_constant (trans_env Σ) kn cst ->
-  (exists n has_deps typ,
-    nth_error Σ n =
-    Some (kn, has_deps, ConstantDecl {| cst_type := typ; cst_body := EAst.cst_body cst |})) \/
-  ((EAst.cst_body cst = Some tBox \/ EAst.cst_body cst = None) /\
-    exists n has_deps typ,
-      nth_error Σ n = Some (kn, has_deps, TypeAliasDecl typ)).
-Proof.
-  unfold ETyping.declared_constant.
-  intros decl.
+  unfold lookup_env, eq_kername.
   induction Σ as [|((kn' & has_deps') & cst') Σ IH]; [easy|].
-  destruct cst'; cbn in *.
-  - destruct (kername_eq_dec _ _) as [->|].
-    + noconf decl.
-      cbn in *.
-      left.
-      eexists 0, has_deps', (cst_type c).
-      now destruct c.
-    + destruct IH as [(n' & typ & cond)|(isbox & n' & typ & cond)].
-      * eassumption.
-      * left.
-        now exists (S n').
-      * right.
-        split; [easy|].
-        now exists (S n').
-  - destruct IH as [(n' & typ & cond)|(isbox & n' & typ & cond)].
-    + eassumption.
-    + left.
-      now exists (S n').
-    + right.
-      split; [easy|].
-      now exists (S n').
-  - destruct (kername_eq_dec _ _) as [->|].
-    + noconf decl.
-      cbn in *.
-      right.
-      split; [destruct o; tauto|].
-      now eexists 0, _, _.
-    + destruct IH as [(n' & typ & cond)|(isbox & n' & typ & cond)].
-      * eassumption.
-      * left.
-        now exists (S n').
-      * right.
-        split; [easy|].
-        now exists (S n').
+  cbn in *.
+  now destruct (kername_eq_dec _ _) as [->|].
+Qed.
+
+Lemma declared_constant_trans_env Σ kn ecst :
+  declared_constant (trans_env Σ) kn ecst ->
+  (exists cst, ecst = trans_cst cst /\ lookup_env Σ kn = Some (ConstantDecl cst)) \/
+  (exists ta, ecst = {| EAst.cst_body := option_map (fun _ => tBox) ta |} /\
+              lookup_env Σ kn = Some (TypeAliasDecl ta)).
+Proof.
+  unfold declared_constant.
+  rewrite lookup_env_trans_env.
+  cbn.
+  intros decl.
+  destruct (lookup_env Σ kn) as [cst|]; cbn in *; [|congruence].
+  destruct cst; cbn in *; [|congruence|]; noconf decl; eauto.
 Qed.
 
 Fixpoint is_dead (rel : nat) (t : term) : bool :=
@@ -437,25 +357,18 @@ Proof.
       * now rewrite IH.
 Qed.
 
-Lemma eval_dearg_single_head Σ mask head args v :
+Lemma dearg_single_masked mask t args :
   #|mask| <= #|args| ->
-  Σ e⊢ dearg_single mask head args ▷ v ->
-  ∑ hdv, Σ e⊢ head ▷ hdv.
+  dearg_single mask t args = mkApps t (masked mask args).
 Proof.
-  revert head args v.
-  induction mask as [|[] mask IH]; intros head args v l ev.
-  - cbn in *.
-    now apply eval_mkApps_head in ev.
-  - destruct args as [|a args]; cbn in *; [easy|].
-    now eapply (IH _ args).
-  - destruct args as [|a args]; cbn in *; [easy|].
-    edestruct (IH (tApp head a) args) as (appv & ev_app).
-    + easy.
-    + exact ev.
-    + now apply eval_tApp_head in ev_app.
+  intros le.
+  induction mask in mask, t, args, le |- *.
+  - now destruct args.
+  - destruct args; [easy|].
+    now destruct a; cbn in *; apply IHmask.
 Qed.
 
-Lemma eval_dearg_lambdas_inv Σ mask Γ inner v :
+Lemma eval_dearg_lambdas_inv {wfl:WcbvFlags} Σ mask Γ inner v :
   env_closed Σ ->
   closed (it_mkLambda_or_LetIn Γ inner) ->
   #|mask| = #|vasses Γ| ->
@@ -492,28 +405,6 @@ Proof.
         now eapply eval_atom.
       * eexists.
         now eapply eval_atom.
-Qed.
-
-Lemma eval_dearg_single_heads mask args Σ hd hd' hdv v :
-  #|mask| <= #|args| ->
-  Σ e⊢ hd ▷ hdv ->
-  Σ e⊢ dearg_single mask hd' args ▷ v ->
-  Σ e⊢ hd' ▷ hdv ->
-  Σ e⊢ dearg_single mask hd args ▷ v.
-Proof.
-  revert hd hd' hdv args v.
-  induction mask as [|[] mask IH]; intros hd hd' hdv args v len ev_hd ev ev_hd';
-    cbn in *.
-  - now eapply eval_mkApps_heads; [|eassumption|eassumption].
-  - now destruct args; cbn in *.
-  - destruct args; cbn in *; [easy|].
-    apply eval_dearg_single_head in ev as ev_app_hd; [|easy].
-    destruct ev_app_hd as (app_hdv & ev_app_hd).
-    eapply IH.
-    + easy.
-    + now eapply eval_tApp_heads; [| |exact ev_app_hd].
-    + eassumption.
-    + easy.
 Qed.
 
 Lemma no_use_subst k t s s' :
@@ -571,21 +462,9 @@ Proof.
       now apply IHAll.
 Qed.
 
-
 Lemma masked_nil {X} mask :
   @masked X mask [] = [].
 Proof. now destruct mask as [|[] ?]. Qed.
-
-Lemma dearg_single_masked mask t args :
-  #|mask| <= #|args| ->
-  dearg_single mask t args = mkApps t (masked mask args).
-Proof.
-  intros le.
-  induction mask in mask, t, args, le |- *.
-  - now destruct args.
-  - destruct args; [easy|].
-    now destruct a; cbn in *; apply IHmask.
-Qed.
 
 Lemma All2_masked {X Y} {T : X -> Y -> Type} xs ys mask :
   All2 T xs ys ->
@@ -599,7 +478,7 @@ Proof.
     + now constructor.
 Qed.
 
-Lemma dearg_lambdas_correct Σ body args mask v :
+Lemma dearg_lambdas_correct {wfl:WcbvFlags} Σ body args mask v :
   env_closed Σ ->
   closed body ->
   Forall (closedn 0) args ->
@@ -1812,6 +1691,22 @@ Proof.
   now apply Forall_is_expanded_cofix_subst.
 Qed.
 
+Lemma lookup_env_Forall {P} Σ kn decl :
+  lookup_env Σ kn = Some decl ->
+  Forall P Σ ->
+  exists b, P (kn, b, decl).
+Proof.
+  intros look all.
+  unfold lookup_env in *.
+  destruct find as [((kn' & b) & decl')|] eqn:find; cbn in *; [|congruence].
+  noconf look.
+  apply find_some in find as (isin & name_eq).
+  unfold eq_kername in *.
+  destruct kername_eq_dec as [->|]; [|congruence].
+  rewrite Forall_forall in all.
+  now eexists; apply all.
+Qed.
+
 Lemma is_expanded_constant Σ kn cst body :
   is_expanded_env Σ ->
   ETyping.declared_constant (trans_env Σ) kn cst ->
@@ -1821,14 +1716,16 @@ Proof.
   intros exp_env decl body_eq.
   unfold is_expanded_env in *.
   apply forallb_Forall in exp_env.
-  eapply declared_constant_trans in decl as [(? & ? & ? & nth)|(is_box & _)].
-  - rewrite body_eq in nth.
-    now eapply nth_error_forall in nth; [|eassumption].
-  - destruct is_box; [|congruence].
+  apply declared_constant_trans_env in decl as [(? & -> & look)|(? & -> & look)]; cbn in *.
+  - eapply lookup_env_Forall in look as (? & P); eauto.
+    destruct x.
+    cbn in *.
+    now rewrite body_eq in P.
+  - destruct x; cbn in *; [|congruence].
     now replace body with tBox by congruence.
 Qed.
 
-Lemma eval_is_expanded_aux Σ t v k :
+Lemma eval_is_expanded_aux {wfl:WcbvFlags} Σ t v k :
   trans_env Σ e⊢ t ▷ v ->
   is_expanded_env Σ ->
   is_expanded_aux k t ->
@@ -2258,12 +2155,13 @@ Lemma valid_cases_constant Σ kn cst body :
   valid_cases body.
 Proof.
   intros valid_env decl_const body_eq.
-  eapply declared_constant_trans in decl_const as [(? & ? & ? & nth)|(is_box & _)].
-  - eapply nth_error_forallb in valid_env.
-    rewrite nth in valid_env.
+  eapply declared_constant_trans_env in decl_const as [(? & -> & look)|(? & -> & look)].
+  - apply forallb_Forall in valid_env.
+    eapply lookup_env_Forall in valid_env as (? & valid); eauto.
+    destruct x.
     cbn in *.
-    now rewrite body_eq in valid_env; propify.
-  - destruct is_box; [|congruence].
+    now rewrite body_eq in valid; propify.
+  - destruct x; cbn in *; [|congruence].
     now replace body with tBox by congruence.
 Qed.
 
@@ -2274,21 +2172,20 @@ Lemma valid_dearg_mask_constant Σ kn cst body :
   valid_dearg_mask (get_const_mask kn) body.
 Proof.
   intros valid_env decl_const body_eq.
-  eapply declared_constant_trans in decl_const as [(? & ? & ? & nth)|(is_box & ? & ? & ? & nth)].
-  - eapply nth_error_forallb in valid_env.
-    rewrite nth in valid_env.
+  apply forallb_Forall in valid_env.
+  eapply declared_constant_trans_env in decl_const as [(? & -> & look)|(? & -> & look)].
+  - eapply lookup_env_Forall in valid_env as (? & valid); eauto.
+    destruct x.
     cbn in *.
-    now rewrite body_eq in valid_env; propify.
-  - eapply nth_error_forallb in valid_env.
-    rewrite nth in valid_env.
-    cbn in *.
-    destruct is_box; [|congruence].
+    now rewrite body_eq in valid; propify.
+  - eapply lookup_env_Forall in valid_env as (? & valid); eauto.
+    destruct x; cbn in *; [|congruence].
     replace body with tBox by congruence.
     cbn.
     now destruct get_const_mask.
 Qed.
 
-Lemma eval_valid_cases Σ t v :
+Lemma eval_valid_cases {wfl:WcbvFlags} Σ t v :
   trans_env Σ e⊢ t ▷ v ->
 
   env_closed (trans_env Σ) ->
@@ -2381,31 +2278,34 @@ Proof with auto with dearg.
   - easy.
 Qed.
 
+Lemma lookup_env_dearg_env Σ kn :
+  lookup_env (dearg_env Σ) kn = option_map (dearg_decl kn) (lookup_env Σ kn).
+Proof.
+  unfold lookup_env.
+  induction Σ as [|((kn', has_deps), decl) Σ IH]; [easy|].
+  cbn.
+  unfold eq_kername.
+  destruct kername_eq_dec as [->|]; [easy|].
+  apply IH.
+Qed.
+
 Lemma declared_constant_dearg Σ k cst :
-  ETyping.declared_constant (trans_env Σ) k cst ->
+  declared_constant (trans_env Σ) k cst ->
   ∑ cst',
-    ETyping.declared_constant (trans_env (dearg_env Σ)) k cst' ×
+    declared_constant (trans_env (dearg_env Σ)) k cst' ×
     EAst.cst_body cst' = option_map (dearg ∘ dearg_lambdas (get_const_mask k))
                                     (EAst.cst_body cst).
 Proof.
-  unfold ETyping.declared_constant.
+  unfold declared_constant.
+  rewrite !lookup_env_trans_env, lookup_env_dearg_env.
   intros typ.
-  induction Σ as [|((kn, has_deps), decl) Σ IH]; [easy|].
-  cbn in *.
-  destruct decl; cbn in *.
-  - destruct (kername_eq_dec k kn) as [->|].
-    + noconf typ.
-      eexists.
-      now split; [reflexivity|].
-    + now apply IH.
-  - now apply IH.
-  - destruct (kername_eq_dec k kn) as [->|].
-    + noconf typ.
-      eexists.
-      split; [reflexivity|].
-      cbn.
-      now destruct o.
-    + now apply IH.
+  destruct lookup_env as [decl|]; cbn in *; [|congruence].
+  destruct decl; cbn in *; [|congruence|]; noconf typ; eauto.
+  cbn.
+  eexists.
+  split; [reflexivity|].
+  cbn.
+  now destruct o.
 Qed.
 
 Inductive dearg_spec : term -> term -> Type :=
@@ -2611,7 +2511,7 @@ Proof.
     right; easy.
 Qed.
 
-Lemma eval_mkApps_tConstruct Σ ind c args argsv
+Lemma eval_mkApps_tConstruct {wfl:WcbvFlags} Σ ind c args argsv
       (a : All2 (eval Σ) args argsv) :
   Σ e⊢ mkApps (tConstruct ind c) args ▷ mkApps (tConstruct ind c) argsv.
 Proof.
@@ -2665,6 +2565,7 @@ Ltac facts :=
      end).
 
 Section dearg.
+  Context {wfl:WcbvFlags}.
   Context (n : nat).
   Context (Σ : global_env).
   Context (clos_Σ : env_closed (trans_env Σ)).
@@ -2980,7 +2881,23 @@ Proof.
         apply filter_length.
 Qed.
 
-Lemma dearg_correct Σ t v :
+Lemma is_propositional_trans_env_dearg_env Σ ind :
+  is_propositional (trans_env (dearg_env Σ)) ind =
+  is_propositional (trans_env Σ) ind.
+Proof.
+  unfold is_propositional.
+  rewrite !lookup_env_trans_env, lookup_env_dearg_env.
+  destruct lookup_env; cbn in *; [|reflexivity].
+  destruct g; cbn in *; auto.
+  rewrite !nth_error_map.
+  unfold dearg_mib.
+  destruct get_mib_masks; [|reflexivity].
+  cbn.
+  rewrite nth_error_mapi.
+  now destruct nth_error.
+Qed.
+
+Lemma dearg_correct {wfl:WcbvFlags} Σ t v :
   env_closed (trans_env Σ) ->
   closed t ->
 
@@ -3005,6 +2922,7 @@ Proof.
   destruct (dearg_elim t).
   - apply is_expanded_aux_mkApps_inv in exp_t as (exp_hd & exp_args).
     cbn in *; propify.
+    rewrite dearg_single_masked by (now rewrite map_length).
     specialize (eval_mkApps_deriv ev) as (? & ev_const & argsv & ev_args & deriv).
     depelim ev_const; cbn in *; [|easy].
     eapply declared_constant_dearg in isdecl as isdecl_dearg.
@@ -3012,14 +2930,14 @@ Proof.
     rewrite e in body_dearg; cbn in *.
 
     enough (trans_env (dearg_env Σ)
-            e⊢ dearg_single (get_const_mask kn)
-                           (dearg (dearg_lambdas (get_const_mask kn) body))
-                           (map dearg args) ▷ dearg v) as ev'.
-    { eapply eval_dearg_single_head in ev' as ev_hd; [|now rewrite map_length].
+            e⊢ mkApps (dearg (dearg_lambdas (get_const_mask kn) body))
+                      (masked (get_const_mask kn) (map dearg args)) ▷ dearg v) as ev'.
+    { eapply eval_mkApps_head in ev' as ev_hd.
       destruct ev_hd as (hdv & ev_hd).
-      eapply eval_dearg_single_heads; try eassumption.
-      - now rewrite map_length.
-      - econstructor; eassumption. }
+      eapply eval_mkApps_heads.
+      3: eassumption.
+      1: eassumption.
+      econstructor; eassumption. }
 
     rewrite dearg_dearg_lambdas by
         eauto using valid_dearg_mask_constant, valid_cases_constant.
@@ -3030,7 +2948,6 @@ Proof.
       - exists ev'.
         now cbn in *. }
 
-    rewrite dearg_single_masked by (now rewrite map_length).
     apply dearg_lambdas_correct.
     + now apply env_closed_dearg.
     + apply closedn_dearg_aux; [|easy].
@@ -3113,6 +3030,7 @@ Proof.
         rewrite dearg_mkApps in *.
         cbn in *.
         now rewrite dearg_single_masked in * by (now rewrite map_length).
+      * rewrite is_propositional_trans_env_dearg_env; eauto.
       * destruct (get_mib_masks _) eqn:mm; cycle 1.
         { cbn in *.
           unfold get_ctor_mask.
@@ -3214,8 +3132,10 @@ Proof.
                           end).
       apply (eval_iota_sing _ _ _ _ _ (n - count_ones branch_mask)
                             (dearg_lambdas branch_mask (dearg f))).
+      * eauto.
       * unshelve eapply (IH _ tBox); eauto.
         lia.
+      * rewrite is_propositional_trans_env_dearg_env; eauto.
       * destruct (get_mib_masks _); cbn in *; [easy|].
         now rewrite dearg_lambdas_nil, Nat.sub_0_r.
       * replace (repeat tBox _) with (masked branch_mask (repeat tBox n)); cycle 1.
@@ -3341,6 +3261,7 @@ Proof.
         rewrite dearg_mkApps in *.
         cbn in *.
         now rewrite dearg_single_masked in * by (now rewrite map_length).
+      * rewrite is_propositional_trans_env_dearg_env; eauto.
       * clear clos_constr valid_constr.
         unfold get_ctor_mask in *.
         revert ev2 deriv_len.
@@ -3383,9 +3304,11 @@ Proof.
       propify.
       destruct valid_hd as (valid_hd & valid_p).
       unfold dearg_proj.
-      apply eval_proj_box.
-      unshelve eapply (IH _ _ _ _ _ ev _); auto.
-      lia.
+      apply eval_proj_prop.
+      * eauto.
+      * unshelve eapply (IH _ _ _ _ _ ev _); auto.
+        lia.
+      * rewrite is_propositional_trans_env_dearg_env; eauto.
     + congruence.
 
   - facts.
@@ -3417,17 +3340,48 @@ Proof.
 Qed.
 End dearg_correct.
 
-Lemma trans_env_debox_env_types Σ :
-  trans_env (debox_env_types Σ) = trans_env Σ.
+Lemma lookup_env_debox_env_types Σ kn :
+  lookup_env (debox_env_types Σ) kn = option_map (debox_type_decl Σ) (lookup_env Σ kn).
 Proof.
-  unfold debox_env_types.
-  generalize Σ at 1 as masks.
-  induction Σ as [|(kn, decl) Σ IH]; intros masks; [easy|].
-  cbn in *.
-  destruct decl; cbn in *.
-  - f_equal.
-    apply IH.
-  - easy.
-  - f_equal.
-    apply IH.
+  unfold debox_env_types, lookup_env.
+  generalize Σ at 1 3.
+  intros masks.
+  induction Σ as [|((kn', has_deps), decl) Σ IH]; [easy|].
+  cbn.
+  unfold eq_kername.
+  destruct kername_eq_dec as [->|]; [easy|].
+  apply IH.
+Qed.
+
+Lemma is_propositional_trans_env_debox_env_types Σ ind :
+  is_propositional (trans_env (debox_env_types Σ)) ind =
+  is_propositional (trans_env Σ) ind.
+Proof.
+  unfold is_propositional.
+  rewrite !lookup_env_trans_env, lookup_env_debox_env_types.
+  destruct lookup_env; cbn in *; [|reflexivity].
+  destruct g; cbn in *; auto.
+  rewrite !nth_error_map.
+  now destruct nth_error.
+Qed.
+
+Lemma eval_debox_env_types {wfl:WcbvFlags} Σ t v :
+  trans_env Σ e⊢ t ▷ v ->
+  trans_env (debox_env_types Σ) e⊢ t ▷ v.
+Proof.
+  induction 1; try solve [econstructor; eauto].
+  - eapply eval_iota; eauto.
+    now rewrite is_propositional_trans_env_debox_env_types.
+  - eapply eval_iota_sing; eauto.
+    now rewrite is_propositional_trans_env_debox_env_types.
+  - eapply eval_delta; eauto.
+    unfold declared_constant in *.
+    rewrite !lookup_env_trans_env, lookup_env_debox_env_types in *.
+    destruct lookup_env; cbn in *; [|congruence].
+    destruct g; cbn in *; auto.
+    congruence.
+  - eapply eval_proj; eauto.
+    now rewrite is_propositional_trans_env_debox_env_types.
+  - eapply eval_proj_prop; eauto.
+    now rewrite is_propositional_trans_env_debox_env_types.
 Qed.
